messageInvariantPrototypes/toyLeaderElection/readme.md
@@ -3,9 +3,20 @@
 The Toy Leader Election Protocol, sourced from "Modularity for Decidability of
 Deductive Verification with Applications to Distributed Systems" (PLDI'18)
 
+There are two favors of this protocol.
+
+## With Atomic Recv-And-Send Steps
+
 1. Client broadcasts StartElection. This is modeled as StartElection message existing in the network at genesis.
 2. A node receiving client request broadcasts Vote-Req, if it has not already voted
 3. A node receiving Vote-Req broadcasts a Vote for the sender, if it has not already voted
 4. A node receiving a quorum of Votes declares itself the leader, broadcasts Leader message
 
-Note that without Monotonic Transformation, the Application Invariant relies on network state.
+## Without Atomic Recv-And-Send Steps
+
+1. Client broadcasts StartElection. This is modeled as StartElection message existing in the network at genesis.
+2. A node receiving client request nominates itself as the candidate, if it does not already have a candidate.
+3. A node with itself as the nominee broadcasts Vote-Req.
+4. A node receiving Vote-Req nominates the sender.
+5. A node with a nominee votes for the nominee.
+6. A node receiving a quorum of Votes declares itself the leader, broadcasts Leader message
